Valaig/Refs.lean
@@ -57,8 +57,12 @@ theorem lt_idx (var var' : Var) :
 
 grind_pattern le_idx => var.idx, var'.idx, var ≤ var'
 grind_pattern le_idx => var.idx, var'.idx, var > var'
+grind_pattern le_idx => var.idx, var'.idx, var.idx ≤ var'.idx
+grind_pattern le_idx => var.idx, var'.idx, var.idx > var'.idx
 grind_pattern lt_idx => var.idx, var'.idx, var < var'
 grind_pattern lt_idx => var.idx, var'.idx, var ≥ var'
+grind_pattern lt_idx => var.idx, var'.idx, var.idx < var'.idx
+grind_pattern lt_idx => var.idx, var'.idx, var.idx ≥ var'.idx
 
 instance : Std.LawfulOrderLT Var := by
   apply Std.LawfulOrderLT.of_le
